Logic/Modal/Standard/Kripke/Morphism.lean
@@ -7,71 +7,85 @@ open Formula
 
 namespace Kripke
 
-class Frame.pMorphism (F₁ : Frame) (F₂ : Frame) (f : F₁.World → F₂.World) where
+class Frame.pMorphism (F₁ F₂ : Frame α) (f : F₁.World → F₂.World) where
   forth : ∀ {w v : F₁.World}, w ≺ v → (f w) ≺ (f v)
   back : ∀ {w : F₁.World}, ∀ {v : F₂.World}, (f w) ≺ v → ∃ u, w ≺ u ∧ f u = v
 
-class Model.pMorphism (M₁ : Model α) (M₂ : Model α) (f : M₁.World → M₂.World) extends Frame.pMorphism M₁.Frame M₂.Frame f where
+class Model.pMorphism (M₁ M₂ : Model α) (f : M₁.World → M₂.World) extends Frame.pMorphism M₁.Frame M₂.Frame f where
   atomic : ∀ {w : M₁.World}, ∀ {a : α}, (M₁.Valuation w a) ↔ (M₂.Valuation (f w) a)
 
 end Kripke
 
-variable {M₁ : Model α} {M₂ : Model α}
-         {F₁ : Frame' α} {F₂ : Frame' α}
-         {f} {p : Formula α} {T : Theory α}
+section
 
-lemma Formula.kripke_satisfies.morphism (hMor : Model.pMorphism M₁ M₂ f) {w} : (w ⊧ p) ↔ ((f w) ⊧ p) := by
+variable {p : Formula α} {T : Theory α}
+
+lemma Formula.kripke_satisfies.morphism
+  {M₁ M₂ : Model α} {f : M₁ → M₂} [morphism : Model.pMorphism M₁ M₂ f]
+  {w : M₁.World} : w ⊧ p ↔ (f w) ⊧ p := by
   induction p using Formula.rec' generalizing w with
   | hatom p =>
     constructor;
-    . apply hMor.atomic |>.mp;
-    . apply hMor.atomic |>.mpr
+    . apply morphism.atomic |>.mp;
+    . apply morphism.atomic |>.mpr
   | hbox p ih =>
     simp;
     constructor;
     . intro h w₂ hw₂;
-      obtain ⟨w₁, ⟨hww₁, e⟩⟩ := hMor.back hw₂;
+      obtain ⟨w₁, ⟨hww₁, e⟩⟩ := morphism.back hw₂;
       have := ih.mp $ h w₁ hww₁;
       subst e;
       assumption;
     . intro h w' hww';
-      exact ih.mpr $ h (f w') $ hMor.forth hww';
+      exact ih.mpr $ h (f w') $ morphism.forth hww';
   | _ => simp_all;
 
-lemma Formula.valid_on_KripkeFrame.morphism (hSur : Function.Surjective f) (hMorF : Frame.pMorphism F₁ F₂ f) : (F₁ ⊧ p) → (F₂ ⊧ p) := by
+lemma Formula.valid_on_KripkeFrame.morphism
+  {F₁ F₂ : Frame α} {f : F₁ → F₂} [morphism : Frame.pMorphism F₁ F₂ f]
+  (hSur : f.Surjective)
+  : F₁ ⊧ p → F₂ ⊧ p := by
   contrapose;
   intro h;
   obtain ⟨V₂, w₂, h⟩ := by simpa [valid_on_KripkeFrame, valid_on_KripkeModel] using h;
 
   simp [valid_on_KripkeFrame, valid_on_KripkeModel];
   obtain ⟨w₁, e⟩ : ∃ w₁, f w₁ = w₂ := by apply hSur;
-  existsi λ w a => V₂ (f w) a, w₁;
+  let V₁ := λ w a => V₂ (f w) a;
+  use V₁, w₁;
   subst e;
-  exact kripke_satisfies.morphism ({
-    forth := by intro w v hwv; apply hMorF.forth hwv,
-    back := by intro w v h; apply hMorF.back h,
-    atomic := by simp_all;
-  }) |>.not.mpr h;
 
-lemma Theory.valid_on_KripkeFrame.morphism (hSur : Function.Surjective f) (hMorF : Frame.pMorphism F₁ F₂ f) : (F₁ ⊧* T) → (F₂ ⊧* T) := by
+  have : Model.pMorphism { Frame := F₁, Valuation := V₁ } { Frame := F₂, Valuation := V₂ } f := {
+    forth := morphism.forth,
+    back := morphism.back,
+    atomic := by simp_all
+  };
+
+  exact kripke_satisfies.morphism.not.mpr h;
+
+
+lemma Theory.valid_on_KripkeFrame.morphism
+  {F₁ F₂ : Frame α} {f : F₁ → F₂} [morphism : Frame.pMorphism F₁ F₂ f]
+  (hSur : Function.Surjective f) : (F₁ ⊧* T) → (F₂ ⊧* T) := by
   simp only [Semantics.realizeSet_iff];
   intro h p hp;
-  exact Formula.valid_on_KripkeFrame.morphism hSur hMorF (h hp);
+  exact Formula.valid_on_KripkeFrame.morphism hSur (h hp);
+
+end
 
 -- TODO: Fix type `α`
-theorem Kripke.undefinability_irreflexive : ¬∃ (Ax : AxiomSet α), (∀ {F : Frame'.{0} α}, (Irreflexive F.Rel) ↔ F ⊧* Ax) := by
+theorem Kripke.undefinability_irreflexive : ¬∃ (Ax : AxiomSet α), (∀ {F : Frame.{0} α}, (Irreflexive F.Rel) ↔ F ⊧* Ax) := by
   by_contra hC;
   obtain ⟨Ax, h⟩ := hC;
 
-  let F₁ : Frame' α := { World := Unit ⊕ Unit, Rel := λ w v => w ≠ v };
-  have hIF₁ : Irreflexive F₁.Rel' := by exact f;
+  let F₁ : Frame α := { World := Unit ⊕ Unit, Rel := λ w v => w ≠ v };
+  have hIF₁ : Irreflexive F₁.Rel' := by simp [Irreflexive]; aesop
 
-  let F₂ : Frame' α := { World := Unit, Rel := λ w v => w = v };
+  let F₂ : Frame α := { World := Unit, Rel := λ w v => w = v };
   have hIF₂ : ¬Irreflexive F₂.Rel' := by simp [Irreflexive]; existsi (); trivial;
 
   let f : F₁.World → F₂.World := λ _ => ();
   have hSur : Function.Surjective f := by simp [Function.Surjective];
-  have hMorF : Frame.pMorphism F₁ F₂ f := {
+  have : Frame.pMorphism F₁ F₂ f := {
     forth := by aesop;
     back := by
       simp [F₁, F₂];
@@ -80,7 +94,7 @@ theorem Kripke.undefinability_irreflexive : ¬∃ (Ax : AxiomSet α), (∀ {F : 
       . intro a; left; use (); intro; contradiction;
   }
 
-  have : Irreflexive F₂.Rel := h.mpr $ Theory.valid_on_KripkeFrame.morphism hSur hMorF (h.mp hIF₁);
+  have : Irreflexive F₂.Rel := h.mpr $ Theory.valid_on_KripkeFrame.morphism hSur (h.mp hIF₁);
   contradiction;
 
 end LO.Modal.Standard
