Logic/Modal/Standard/Kripke/Reducible.lean
@@ -6,21 +6,21 @@ namespace LO.Modal.Standard
 namespace Kripke
 
 variable
-  {α : Type u} [DecidableEq α]
+  {α : Type*} [DecidableEq α]
   {L₁ L₂ : DeductionParameter α} [L₁.HasNec] [L₂.HasNec]
-  {P₁ P₂ : FrameProperty}
+  {P₁ P₂ : FrameCondition α}
   [sound₁ : Sound L₁ 𝔽(Ax(L₁))] [sound₂ : Sound L₂ 𝔽(Ax(L₂))]
   [complete₁ : Complete L₁ 𝔽(Ax(L₁))] [complete₂ : Complete L₂ 𝔽(Ax(L₂))]
-  [definability₁ : Definability Ax(L₁) P₁] [definability₂ : Definability Ax(L₂) P₂]
+  (definability₁ : Definability Ax(L₁) P₁) (definability₂ : Definability Ax(L₂) P₂)
 
-lemma reducible_of_subset_axiomSetFrameClass (hs : ∀ {F}, F ∈ 𝔽(Ax(L₂)) → F ∈ 𝔽(Ax(L₁))) : L₁ ≤ₛ L₂ := by
+lemma reducible_of_subset_axiomSetFrameClass (hs : ∀ {F : Frame α}, F ∈ 𝔽(Ax(L₂)) → F ∈ 𝔽(Ax(L₁))) : L₁ ≤ₛ L₂ := by
   apply System.reducible_iff.mpr;
   intro p hp;
   apply complete₂.complete;
   intro F hF;
   exact sound₁.sound hp F $ hs hF;
 
-lemma reducible_of_definability (hs : ∀ {F : Frame}, P₂ F → P₁ F) : L₁ ≤ₛ L₂ := by
+lemma reducible_of_definability (hs : ∀ {F}, P₂ F → P₁ F) : L₁ ≤ₛ L₂ := by
   apply reducible_of_subset_axiomSetFrameClass;
   intro F hF;
   apply iff_definability_memAxiomSetFrameClass definability₁ |>.mpr;
@@ -38,7 +38,7 @@ lemma equiv_of_eq_axiomSetFrameClass
 lemma equiv_of_iff_definability (h : ∀ {F}, P₁ F ↔ P₂ F) : L₁ =ₛ L₂ := by
   apply System.Equiv.antisymm_iff.mpr;
   constructor;
-  . apply reducible_of_definability (definability₁ := definability₁) (definability₂ := definability₂); intros; exact h.mpr (by assumption)
-  . apply reducible_of_definability (definability₁ := definability₂) (definability₂ := definability₁); intros; exact h.mp (by assumption)
+  . apply reducible_of_definability definability₁ definability₂; intros; exact h.mpr (by assumption)
+  . apply reducible_of_definability definability₂ definability₁; intros; exact h.mp (by assumption)
 
 end LO.Modal.Standard.Kripke
